src/Dafny/ExternalTest.dfy
@@ -1,0 +1,11 @@
+module MyWrapper {
+  // The first argument is the class name, the second is the method name
+  method {:extern "ExternalUtils", "NativeMethod"} NativeMethod(x: int) returns (y: int)
+
+    class ExternalTest {
+        method Test() returns (result: int) {
+            result := NativeMethod(42);
+        }
+    }
+
+}
